test/artifact/lib/Hacl.Policies.fst
@@ -17,13 +17,12 @@ module H32  = Hacl.UInt32
 module H64  = Hacl.UInt64
 module H128  = Hacl.UInt128
 
-assume new type declassifiable (#a:Type0) (b:a)
+assume new type declassifiable (x:uint8_p)
 
-
-assume val declassify_u8: x:H8.t{declassifiable x} -> Tot (y:U8.t{H8.v x = U8.v y})
-assume val declassify_u32: x:H32.t{declassifiable x} -> Tot (y:U32.t{H32.v x = U32.v y})
-assume val declassify_u64: x:H64.t{declassifiable x} -> Tot (y:U64.t{H64.v x = U64.v y})
-assume val declassify_u128: x:H128.t{declassifiable x} -> Tot (y:U128.t{H128.v x = U128.v y})
+assume val declassify_u8: x:H8.t -> Tot (y:U8.t{H8.v x = U8.v y})
+assume val declassify_u32: x:H32.t -> Tot (y:U32.t{H32.v x = U32.v y})
+assume val declassify_u64: x:H64.t -> Tot (y:U64.t{H64.v x = U64.v y})
+assume val declassify_u128: x:H128.t -> Tot (y:U128.t{H128.v x = U128.v y})
 
 
 assume val leak_byte:
